cryptoffi revamp. make hasher the primitive, and prove hash on top. make sig, vrf key ownership persistent, to allow for parallel ops. specify vrf correctness, needed to prove server. and tighten spec justifications

external/Goose/github_com/mit_pdos/pav/cryptoffi.v
@@ -5,56 +5,62 @@ Notation SigPublicKey := (slice.T byteT) (only parsing).
 Section code.
 Context `{ext_ty: ext_types}.
 
+(* Hash. *)
+
 Definition HashLen : expr := #32.
 
-Definition Hash: val :=
-  rec: "Hash" "data" :=
-    Panic "ffi";;
-    #().
+Definition NewHasher: val :=
+  rec: "NewHasher" <> :=
+    Panic "ffi".
+
+Definition Hasher__Write: val :=
+  rec: "Hasher__Write" "ptr_hr" "sl_b" :=
+    Panic "ffi".
+
+Definition Hasher__Sum: val :=
+  rec: "Hasher__Sum" "ptr_hr" "sl_b" :=
+    Panic "ffi".
+
+(* Signature. *)
 
 Definition SigGenerateKey: val :=
   rec: "SigGenerateKey" <> :=
-    Panic "ffi";;
-    #().
+    Panic "ffi".
 
 Definition SigPrivateKey__Sign: val :=
   rec: "SigPrivateKey__Sign" "sk" "message" :=
-    Panic "ffi";;
-    #().
+    Panic "ffi".
 
 Definition SigPublicKey__Verify: val :=
   rec: "SigPublicKey__Verify" "pk" "message" "sig" :=
-    Panic "ffi";;
-    #().
+    Panic "ffi".
+
+(* Verifiable Random Function (VRF). *)
 
 Definition VrfGenerateKey: val :=
   rec: "VrfGenerateKey" <> :=
-    Panic "ffi";;
-    #().
+    Panic "ffi".
 
-Definition VrfPrivateKey__Hash: val :=
-  rec: "VrfPrivateKey__Hash" "sk" "data" :=
-    Panic "ffi";;
-    #().
+Definition VrfPrivateKey__Prove: val :=
+  rec: "VrfPrivateKey__Prove" "sk" "data" :=
+    Panic "ffi".
 
 Definition VrfPublicKey__Verify: val :=
   rec: "VrfPublicKey__Verify" "pk" "data" "proof" :=
-    Panic "ffi";;
-    #().
+    Panic "ffi".
 
 Definition VrfPublicKeyEncode: val :=
   rec: "VrfPublicKeyEncode" "pk" :=
-    Panic "ffi";;
-    #().
+    Panic "ffi".
 
 Definition VrfPublicKeyDecode: val :=
   rec: "VrfPublicKeyDecode" "b" :=
-    Panic "ffi";;
-    #().
+    Panic "ffi".
+
+(* Random. *)
 
 Definition RandBytes: val :=
   rec: "RandBytes" "n" :=
-    Panic "ffi";;
-    #().
+    Panic "ffi".
 
 End code.
