src/program_proof/pav/cryptoffi.v
@@ -21,10 +21,6 @@ Proof. Admitted.
 Instance is_hash_timeless data hash : Timeless (is_hash data hash).
 Proof. Admitted.
 
-Lemma is_hash_det d h1 h2 :
-  is_hash d h1 -∗ is_hash d h2 -∗ ⌜h1 = h2⌝.
-Proof. Admitted.
-
 Lemma is_hash_inj d1 d2 h :
   is_hash d1 h -∗ is_hash d2 h -∗ ⌜d1 = d2⌝.
 Proof. Admitted.
@@ -33,30 +29,62 @@ Lemma is_hash_len d h :
   is_hash d h -∗ ⌜length h = hash_len⌝.
 Proof. Admitted.
 
-Lemma wp_Hash sl_data data :
+Definition own_hasher (ptr : loc) (data : list w8) : iProp Σ. Admitted.
+
+Lemma wp_NewHasher :
+  {{{ True }}}
+  NewHasher #()
   {{{
-    "Hdata" ∷ own_slice_small sl_data byteT (DfracOwn 1) data
+    ptr_hr, RET #ptr_hr;
+    "Hown_hr" ∷ own_hasher ptr_hr []
+  }}}.
+Proof. Admitted.
+
+Lemma wp_Hasher__Write sl_b ptr_hr data d0 b :
+  {{{
+    "Hown_hr" ∷ own_hasher ptr_hr data ∗
+    "Hsl_b" ∷ own_slice_small sl_b byteT d0 b
   }}}
-  Hash (slice_val sl_data)
+  Hasher__Write #ptr_hr (slice_val sl_b)
   {{{
-    sl_hash hash, RET (slice_val sl_hash);
-    "Hdata" ∷ own_slice_small sl_data byteT (DfracOwn 1) data ∗
-    "Hhash" ∷ own_slice_small sl_hash byteT (DfracOwn 1) hash ∗
+    RET #();
+    "Hown_hr" ∷ own_hasher ptr_hr (data ++ b) ∗
+    "Hsl_b" ∷ own_slice_small sl_b byteT d0 b
+  }}}.
+Proof. Admitted.
+
+Lemma wp_Hasher__Sum sl_b_in ptr_hr data b_in :
+  {{{
+    "Hown_hr" ∷ own_hasher ptr_hr data ∗
+    "Hsl_b_in" ∷ own_slice sl_b_in byteT (DfracOwn 1) b_in
+  }}}
+  Hasher__Sum #ptr_hr (slice_val sl_b_in)
+  {{{
+    sl_b_out hash, RET (slice_val sl_b_out);
+    "Hown_hr" ∷ own_hasher ptr_hr data ∗
+    "Hsl_b_out" ∷ own_slice sl_b_out byteT (DfracOwn 1) (b_in ++ hash) ∗
     "#His_hash" ∷ is_hash data hash
   }}}.
 Proof. Admitted.
 
 (* Signatures. *)
 
-(* own_sig_sk says that an sk is in-distribution.
-sk is a ptr bc the actual sk never leaves the ffi.
-this prevents code from accidentally leaking it.
-pk is a mathematical list bc it could potentially be shared,
-altho our app doesn't make use of that. *)
-Definition own_sig_sk (ptr_sk : loc) (pk : list w8) (P : list w8 → iProp Σ) : iProp Σ.
+(* is_sig_sk says that an sk is in-distribution.
+furthermore, it came from calling the Generate fn,
+and the underlying sk is enclosed in the ffi,
+forcing all users to establish the sigpred.
+pk is a mathematical list so it can leave the ffi and be sent
+between parties. *)
+Definition is_sig_sk (ptr_sk : loc) (pk : list w8) (P : list w8 → iProp Σ) : iProp Σ.
 Admitted.
 
-(* is_sig_pk says that a pk is in-distribution. *)
+#[global]
+Instance is_sig_sk_persistent ptr_sk pk P : Persistent (is_sig_sk ptr_sk pk P).
+Proof. Admitted.
+
+(* is_sig_pk says that pk is in-distribution.
+also, that it came from the Generate fn,
+tied by P to a corresponding sk in the ffi. *)
 Definition is_sig_pk (pk : list w8) (P : list w8 → iProp Σ) : iProp Σ.
 Admitted.
 
@@ -74,7 +102,7 @@ Admitted.
 Instance is_sig_persistent pk msg sig : Persistent (is_sig pk msg sig).
 Proof. Admitted.
 
-(* is_sig_to_pred has two cases:
+(* the proof for is_sig_to_pred splits into two cases:
 1) the sig came from sign. P clearly holds.
 2) an adversary forged the sig.
 EUF-CMA guarantees that this only happens if the genuine key holder
@@ -93,27 +121,26 @@ Lemma wp_SigGenerateKey P :
     sl_pk pk ptr_sk, RET ((slice_val sl_pk), #ptr_sk);
     "Hsl_sig_pk" ∷ own_slice_small sl_pk byteT (DfracOwn 1) pk ∗
     "#His_sig_pk" ∷ is_sig_pk pk P ∗
-    "Hown_sig_sk" ∷ own_sig_sk ptr_sk pk P
+    "#His_sig_sk" ∷ is_sig_sk ptr_sk pk P
  }}}.
 Proof. Admitted.
 
 Lemma wp_SigPrivateKey__Sign ptr_sk pk P sl_msg msg d0 :
   {{{
-    "Hown_sig_sk" ∷ own_sig_sk ptr_sk pk P ∗
+    "#His_sig_sk" ∷ is_sig_sk ptr_sk pk P ∗
     "HP" ∷ P msg ∗
     "Hsl_msg" ∷ own_slice_small sl_msg byteT d0 msg
   }}}
   SigPrivateKey__Sign #ptr_sk (slice_val sl_msg)
   {{{
     sl_sig (sig : list w8), RET (slice_val sl_sig);
-    "Hown_sig_sk" ∷ own_sig_sk ptr_sk pk P ∗
     "Hmsg" ∷ own_slice_small sl_msg byteT d0 msg ∗
     "Hsl_sig" ∷ own_slice_small sl_sig byteT (DfracOwn 1) sig ∗
     "#His_sig" ∷ is_sig pk msg sig
   }}}.
 Proof. Admitted.
 
-Lemma wp_SigPublicKey__Verify P sl_pk pk sl_sig sl_msg (sig msg : list w8) d0 d1 d2 :
+Lemma wp_SigPublicKey__Verify sl_pk pk sl_sig sl_msg (sig msg : list w8) d0 d1 d2 :
   {{{
     "Hsl_pk" ∷ own_slice_small sl_pk byteT d0 pk ∗
     "Hsl_sig" ∷ own_slice_small sl_sig byteT d1 sig ∗
@@ -125,40 +152,49 @@ Lemma wp_SigPublicKey__Verify P sl_pk pk sl_sig sl_msg (sig msg : list w8) d0 d1
     "Hsl_pk" ∷ own_slice_small sl_pk byteT d0 pk ∗
     "Hsl_sig" ∷ own_slice_small sl_sig byteT d1 sig ∗
     "Hsl_msg" ∷ own_slice_small sl_msg byteT d2 msg ∗
-    "Hgenie" ∷ (is_sig pk msg sig ∗-∗ ⌜ err = false ⌝) ∗
-    (* TODO: remove. subsumed by is_sig_to_pred. *)
-    "HP" ∷ (is_sig_pk pk P -∗ if negb err then P msg else True)
+    "Hgenie" ∷ (is_sig pk msg sig -∗ ⌜ err = false ⌝) ∗
+    "Herr" ∷ (⌜ err = false ⌝ -∗ is_sig pk msg sig)
   }}}.
 Proof. Admitted.
 
 (* Verifiable Random Functions (VRFs).
-our model omits the following, since they're not needed in KT.
-- a data predicate. this allows the sk owner to prove that hashed
-  data satisfies some properties.
-- correctness.
-- injectivity. *)
+we model "Full Uniqueness" (from the IETF spec) and correctness.
+we omit "Full Collision Resistance", since it's not needed in KT. *)
 
-(* own_vrf_sk provides ownership of an sk from the VrfGenerateKey function. *)
-Definition own_vrf_sk (ptr_sk : loc) : iProp Σ.
-Admitted.
-
-(* own_vrf_pk provides enough resources for pk_ptr, and says that
-pk satisfies certain crypto checks.
-however, pk might still be from outside the VrfGenerateKey distribution. *)
-Definition own_vrf_pk (ptr_pk : loc) (pk : list w8) : iProp Σ.
-Admitted.
-
-(* is_vrf says that for a particular pk, data and hash are tied together,
-through the Verify function. *)
-Definition is_vrf (pk : list w8) (data : list w8) (hash : list w8) : iProp Σ.
+(* is_vrf_sk provides ownership of an sk from the VrfGenerateKey function. *)
+Definition is_vrf_sk (ptr_sk : loc) (pk : list w8) : iProp Σ.
 Admitted.
 
 #[global]
-Instance is_vrf_persistent pk data hash : Persistent (is_vrf pk data hash).
+Instance is_vrf_sk_persistent ptr_sk pk : Persistent (is_vrf_sk ptr_sk pk).
 Proof. Admitted.
 
-Lemma is_vrf_det pk d h1 h2 :
-  is_vrf pk d h1 -∗ is_vrf pk d h2 -∗ ⌜h1 = h2⌝.
+(* is_vrf_pk says that pk satisfies certain mathematical crypto checks.
+this is in contrast to is_sig_pk, which additionally says that
+the corresponding sk never left the ffi. *)
+Definition is_vrf_pk (ptr_pk : loc) (pk : list w8) : iProp Σ.
+Admitted.
+
+#[global]
+Instance is_vrf_pk_persistent ptr_pk pk : Persistent (is_vrf_pk ptr_pk pk).
+Proof. Admitted.
+
+(* is_vrf says that for a particular pk, data and out are tied together,
+through the Verify function. *)
+Definition is_vrf (pk : list w8) (data : list w8) (out : list w8) : iProp Σ.
+Admitted.
+
+#[global]
+Instance is_vrf_persistent pk data out : Persistent (is_vrf pk data out).
+Proof. Admitted.
+
+(* VRFs give deterministic outputs, aka, "Full Uniqueness" from IETF spec. *)
+Lemma is_vrf_det pk d o1 o2 :
+  is_vrf pk d o1 -∗ is_vrf pk d o2 -∗ ⌜o1 = o2⌝.
+Proof. Admitted.
+
+Lemma is_vrf_len pk d o :
+  is_vrf pk d o -∗ ⌜ length o = hash_len ⌝.
 Proof. Admitted.
 
 Lemma wp_VrfGenerateKey :
@@ -166,46 +202,46 @@ Lemma wp_VrfGenerateKey :
   VrfGenerateKey #()
   {{{
     (ptr_pk ptr_sk : loc) (pk : list w8), RET (#ptr_pk, #ptr_sk);
-    "Hown_vrf_pk" ∷ own_vrf_pk ptr_pk pk ∗
-    "Hown_vrf_sk" ∷ own_vrf_sk ptr_sk
+    "#His_vrf_pk" ∷ is_vrf_pk ptr_pk pk ∗
+    "#His_vrf_sk" ∷ is_vrf_sk ptr_sk pk
   }}}.
 Proof. Admitted.
 
-Lemma wp_VrfPrivateKey__Hash (ptr_sk : loc) sl_data (data : list w8) d0 :
+Lemma wp_VrfPrivateKey__Prove ptr_sk pk sl_data (data : list w8) d0 :
   {{{
-    "Hown_vrf_sk" ∷ own_vrf_sk ptr_sk ∗
+    "#His_vrf_sk" ∷ is_vrf_sk ptr_sk pk ∗
     "Hsl_data" ∷ own_slice_small sl_data byteT d0 data
   }}}
-  VrfPrivateKey__Hash #ptr_sk (slice_val sl_data)
+  VrfPrivateKey__Prove #ptr_sk (slice_val sl_data)
   {{{
-    sl_hash sl_proof (hash proof : list w8), RET (slice_val sl_hash, slice_val sl_proof);
-    "Hown_vrf_sk" ∷ own_vrf_sk ptr_sk ∗
+    sl_out sl_proof (out proof : list w8), RET (slice_val sl_out, slice_val sl_proof);
     "Hsl_data" ∷ own_slice_small sl_data byteT d0 data ∗
-    "Hsl_hash" ∷ own_slice_small sl_hash byteT (DfracOwn 1) hash ∗
-    "Hsl_proof" ∷ own_slice_small sl_proof byteT (DfracOwn 1) proof
+    "Hsl_out" ∷ own_slice_small sl_out byteT (DfracOwn 1) out ∗
+    "Hsl_proof" ∷ own_slice_small sl_proof byteT (DfracOwn 1) proof ∗
+    "#His_vrf" ∷ is_vrf pk data out
   }}}.
 Proof. Admitted.
 
 Lemma wp_VrfPublicKey__Verify ptr_pk pk sl_data sl_proof (data proof : list w8) d0 d1 :
   {{{
-    "Hown_vrf_pk" ∷ own_vrf_pk ptr_pk pk ∗
+    "#His_vrf_pk" ∷ is_vrf_pk ptr_pk pk ∗
     "Hsl_data" ∷ own_slice_small sl_data byteT d0 data ∗
     "Hsl_proof" ∷ own_slice_small sl_proof byteT d1 proof
   }}}
   VrfPublicKey__Verify #ptr_pk (slice_val sl_data) (slice_val sl_proof)
   {{{
-    sl_hash (hash : list w8) (err : bool), RET (slice_val sl_hash, #err);
-    "Hown_vrf_pk" ∷ own_vrf_pk ptr_pk pk ∗
+    sl_out (out : list w8) (err : bool), RET (slice_val sl_out, #err);
     "Hsl_data" ∷ own_slice_small sl_data byteT d0 data ∗
     "Hsl_proof" ∷ own_slice_small sl_proof byteT d1 proof ∗
-    "Hsl_hash" ∷ own_slice_small sl_hash byteT (DfracOwn 1) hash ∗
-    "#His_vrf" ∷ (if negb err then is_vrf pk data hash else True)
+    "Hsl_out" ∷ own_slice_small sl_out byteT (DfracOwn 1) out ∗
+    "Hgenie" ∷ (is_vrf pk data out -∗ ⌜ err = false ⌝) ∗
+    "Herr" ∷ (⌜ err = false ⌝ -∗ is_vrf pk data out)
   }}}.
 Proof. Admitted.
 
 Lemma wp_VrfPublicKeyEncode ptr_pk pk :
   {{{
-    "Hown_vrf_pk" ∷ own_vrf_pk ptr_pk pk
+    "His_vrf_pk" ∷ is_vrf_pk ptr_pk pk
   }}}
   VrfPublicKeyEncode #ptr_pk
   {{{
@@ -222,7 +258,7 @@ Lemma wp_VrfPublicKeyDecode sl_enc pk d0 :
   {{{
     (ptr_pk : loc), RET #ptr_pk;
     "Hsl_enc" ∷ own_slice_small sl_enc byteT d0 pk ∗
-    "Hown_vrf_pk" ∷ own_vrf_pk ptr_pk pk
+    "His_vrf_pk" ∷ is_vrf_pk ptr_pk pk
   }}}.
 Proof. Admitted.
 
